Working on part of certiL1g_to_L2Correct that Abhishek left unfinished.

certicoq/theories/L1g/instances.v
@@ -5,47 +5,52 @@ Require Import Common.Common.
 Require Import Common.classes.
 Require Import certiClasses2.
 
-Instance bigStepOpSemL1gTerm : BigStepOpSem (Program L1g.compile.Term) :=
+Instance bigStepOpSemL1gTerm: BigStepOpSem (Program L1g.compile.Term) :=
   BigStepOpWEnv _ WcbvEval.
 
 (** FIX!! *)
-Instance WfL1gTerm : GoodTerm (Program L1g.compile.Term) :=
+Instance WfL1gTerm: GoodTerm (Program L1g.compile.Term) :=
   fun _  => True.
 
 Require Import SquiggleEq.UsefulTypes.
 Require Import DecidableClass.
 
-Definition flattenApp (t:L1g.compile.Term) : (L1g.compile.Term * (list L1g.compile.Term)).
-Admitted.
+Definition flattenApp (t:L1g.compile.Term):
+  (L1g.compile.Term * (list L1g.compile.Term)) :=
+  match t with
+    | TApp fn arg args => (fn, cons arg (Terms_list args))
+    | s => (s, nil)
+  end.
 
-Global Instance QuestionHeadL2Term : QuestionHead (Program L1g.compile.Term) :=
-fun q t =>
-match q, fst (flattenApp (main t)) with
-| Cnstr ind ci, TConstruct ind2 ci2 _(*nargs*) =>
-  andb (decide (ind=ind2)) (decide (ci=ci2))
-| Abs, TLambda _ _ _ => true
-| _, _ => false 
-end.
+Global Instance QuestionHeadL2Term: QuestionHead (Program L1g.compile.Term) :=
+  fun q t =>
+    match q, fst (flattenApp (main t)) with
+      | Cnstr ind ci, TConstruct ind2 ci2 _(*nargs*) =>
+        andb (decide (ind=ind2)) (decide (ci=ci2))
+      | Abs, TLambda _ _ _ => true
+      | _, _ => false 
+    end.
 
-Global Instance ObsSubtermL2Term : ObserveNthSubterm (Program L1g.compile.Term) :=
-fun n t =>
-match  (flattenApp (main t)) with
-| (TConstruct _ _ _ , subterms) =>
-  match List.nth_error subterms  n with
-  | Some st => Some {| env := env t; main := st |}
-  | None => None
-  end
-| _ => None
-end.
+Global Instance ObsSubtermL2Term:
+  ObserveNthSubterm (Program L1g.compile.Term) :=
+  fun n t =>
+    match  (flattenApp (main t)) with
+      | (TConstruct _ _ _ , subterms) =>
+        match List.nth_error subterms  n with
+          | Some st => Some {| env := env t; main := st |}
+          | None => None
+        end
+      | _ => None
+    end.
 
 
 
-Instance certiL1g : CerticoqLanguage (Program L1g.compile.Term):= {}.
+Instance certiL1g: CerticoqLanguage (Program L1g.compile.Term):= {}.
 
 Local Generalizable Variable Lj.
 
 Definition translateTo `{CerticoqTranslation (Program L1g.compile.Term) Lj}
-  (p:program) : exception Lj :=
+  (p:program): exception Lj :=
   let l1g:= L1g.compile.program_Program p in
   translate (Program L1g.compile.Term) Lj l1g.
 
@@ -55,9 +60,9 @@ Arguments translateTo Lj {H} p.
 Require Import certiClasses.
 
 Definition ctranslateTo {Term Value BigStep WF QH ObsS } 
-  (Lj : @CerticoqLanguage Term Value BigStep WF QH ObsS)
+  (Lj: @CerticoqLanguage Term Value BigStep WF QH ObsS)
    `{CerticoqTranslation (Program L1g.compile.Term) (cTerm Lj)}
-   : program -> exception (cTerm Lj) :=
+  : program -> exception (cTerm Lj) :=
   translateTo (cTerm Lj).
 
 Arguments ctranslateTo {Term0} {Value} {BigStep} {WF} {QH} {ObsS} Lj {H} p.
