certicoq/theories/L2_typeStripped/instances.v
@@ -4,47 +4,54 @@ Require Import certiClasses.
 Require Import Common.Common.
 Require Import L1g.instances.
 Require Import certiClasses2.
+Require Import stripEvalCommute.
 
-Instance bigStepOpSemL2Term : BigStepOpSem (Program L2.compile.Term) :=
+Instance bigStepOpSemL2Term: BigStepOpSem (Program L2.compile.Term) :=
   BigStepOpWEnv _ WcbvEval.
 
-(** If the compiler only correctly compiles terms with some properties, add them here. *)
-Instance WfL2Term : GoodTerm (Program L2.compile.Term) :=
+(** If the compiler only correctly compiles terms with some properties,
+ add them here. *)
+Instance WfL2Term: GoodTerm (Program L2.compile.Term) :=
   fun _  => True.
 
 
 Require Import SquiggleEq.UsefulTypes.
 Require Import DecidableClass.
 
-Definition flattenApp (t:L2.compile.Term) : (L2.compile.Term * (list L2.compile.Term)).
-Admitted.
+Definition flattenApp (t:L2.compile.Term) :
+  (L2.compile.Term * (list L2.compile.Term)) :=
+  match t with
+    | TApp fn arg args => (fn, cons arg (Terms_list args))
+    | s => (s, nil)
+  end.
 
-Global Instance QuestionHeadL2Term : QuestionHead (Program L2.compile.Term) :=
-fun q t =>
-match q, fst (flattenApp (main t)) with
-| Cnstr ind ci, TConstruct ind2 ci2 _(*nargs*) =>
-  andb (decide (ind=ind2)) (decide (ci=ci2))
-| Abs, TLambda _ _ => true
-| _, _ => false 
-end.
+Global Instance QuestionHeadL2Term: QuestionHead (Program L2.compile.Term) :=
+  fun q t =>
+    match q, fst (flattenApp (main t)) with
+      | Cnstr ind ci, TConstruct ind2 ci2 _(*nargs*) =>
+        andb (decide (ind=ind2)) (decide (ci=ci2))
+      | Abs, TLambda _ _ => true
+      | _, _ => false 
+    end.
 
-Global Instance ObsSubtermL2Term : ObserveNthSubterm (Program L2.compile.Term) :=
-fun n t =>
-match  (flattenApp (main t)) with
-| (TConstruct _ _ _ , subterms) =>
-  match List.nth_error subterms  n with
-  | Some st => Some {| env := env t; main := st |}
-  | None => None
-  end
-| _ => None
-end.
+Global Instance ObsSubtermL2Term :
+  ObserveNthSubterm (Program L2.compile.Term) :=
+  fun n t =>
+    match  (flattenApp (main t)) with
+      | (TConstruct _ _ _ , subterms) =>
+        match List.nth_error subterms  n with
+          | Some st => Some {| env := env t; main := st |}
+          | None => None
+        end
+      | _ => None
+    end.
 
-Global Instance certiL2Eval : BigStepOpSem (Program L2.compile.Term).
+Global Instance certiL2Eval: BigStepOpSem (Program L2.compile.Term).
   apply BigStepOpWEnv.
   apply WcbvEval.
 Defined.
 
-Global Instance certiL2 : CerticoqLanguage (Program L2.compile.Term).
+Global Instance certiL2: CerticoqLanguage (Program L2.compile.Term).
 
 Instance certiL1g_to_L2: 
   CerticoqTotalTranslation (Program L1g.compile.Term)
@@ -55,17 +62,28 @@ Instance certiL1g_to_L2:
 Require Import certiClasses2.
 
 
-Global Instance certiL1g_to_L2Correct :  CerticoqTranslationCorrect certiL1g certiL2.
+Global Instance certiL1g_to_L2Correct :
+  CerticoqTranslationCorrect certiL1g certiL2.
 Proof.
   split.
-  - intros ? ?. simpl. unfold translateT, certiL1g_to_L2.
-    (* The GoodTerm instance of  L1g and L2 may need to be strengthened to complete the next
-      subgoal. Currently, they evaluete to True, which is trivial.
-      unfold goodTerm in *. 
-
-     *) admit.
+  - intros ? ?. cbn. unfold translateT, certiL1g_to_L2. trivial.
+    (* The GoodTerm instance of L1g and L2 may need to be strengthened 
+       to complete the next subgoal. Currently, they evaluete to True.
+     *)
   - intros ? ?. 
     repeat progress (unfold bigStepEval, bigStepEvalSame,
-                     liftBigStepException, bigStepOpSemL1gTerm, translate, translateT, BigStepOpWEnv,
-                     liftTotal, certiL2Eval, certiL1g_to_L2). simpl.
+                     liftBigStepException, bigStepOpSemL1gTerm,
+                     translate, translateT, BigStepOpWEnv,
+                     liftTotal, certiL2Eval, certiL1g_to_L2).
+    cbn. intros. destruct H0.
+    exists (stripProgram sv). cbn. repeat split.
+    + apply (proj1 (stripEvalCommute.WcbvEval_hom (env s)) _ _ H0).
+    + destruct s, sv. cbn in H1. rewrite H1. cbn. reflexivity.
+    + admit.
+    + intros. unfold observeNthSubterm,
+              ObsSubtermL2Term, instances.ObsSubtermL2Term.
+      destruct sv. cbn. unfold flattenApp, instances.flattenApp.
+      induction main; cbn; try constructor.
+      *
+
 Admitted.    
